hax-lib/proof-libs/lean/Hax.lean
@@ -1,0 +1,4 @@
+-- This module serves as the root of the `Hax` library.
+-- Import modules here that should be built as part of the library.
+import Hax.BitVec
+import Hax.Lib
