hax-lib/proof-libs/lean/Hax/BitVec.lean
@@ -1,0 +1,17 @@
+
+
+namespace BitVec
+
+@[simp]
+theorem toNat_mul_iff_not_umulOverflow {w} {x y : BitVec w} :
+    w > 0 →
+    ((x * y).toNat = x.toNat * y.toNat ↔ (¬ umulOverflow x y)) := by
+  intros h_w
+  constructor <;> try apply toNat_mul_of_not_umulOverflow
+  intros h
+  simp only [umulOverflow, ge_iff_le, decide_eq_true_eq, Nat.not_le] at *
+  simp [toNat_mul, Nat.mod_eq_iff_lt] at *
+  assumption
+
+
+end BitVec
