hax-lib/proof-libs/lean/README.md
@@ -1,0 +1,7 @@
+# Hax Lean library
+
+This folder contains the Lean library necessary to use hax-extracted rust code
+in Lean. It is organized as follows:
+
+- `Lib.lean` : main prelude definitions (integer types, arrays, errors, etc)
+- `BitVec.lean` : additional lemmas and tactics to handle bitvectors
